Clearer naming

generic.v
@@ -9,9 +9,21 @@ Require Import univ utils.
 
 (* Generic Library *)
 
-(****** Type specialization ******)
+(* Most of the type signatures and the general structure of the library from
+    Weirich + Casinghino
+    - https://dl.acm.org/doi/pdf/10.1145/1707790.1707799
+    Which itself is largely based on the generic library by Verbruggen et al.:
+    - https://dl.acm.org/doi/pdf/10.1145/1411318.1411326 *)
+
+(* Main differences in the usage of universepolymorfism
+   and the curiosities of Coq with regards to getting the definitions
+   to actually typecheck. *)
+
+(****** Type level definitions ******)
 Section types.
 
+(* A kind-indexed type.
+   Needed for specializing types. *)
 Fixpoint kit (n : nat) (k : kind) (b : vec Type (S n) -> Type)
   : vec (decodeKind k) (S n) -> Type :=
     match k return vec (decodeKind k) (S n) -> Type with
@@ -20,7 +32,8 @@ Fixpoint kit (n : nat) (k : kind) (b : vec Type (S n) -> Type)
                                                kit k2 b (zap vs As))
     end.
 
-(* type for mapping constants to a value *)
+(* Type for mapping constants to a value.
+   Needed for the type signature of specTerm. *)
 Definition tyConstEnv (n : nat) (b : vec Type (S n) -> Type) : Type :=
   forall (k:kind) (c:const k), kit k b (repeat _ (decodeClosed (Con _ c))).
 
@@ -29,19 +42,20 @@ End types.
 (****** Term specialization ******)
 Section terms.
 
-  (* env of kind-indexed types *)
-  Inductive ngenv (n : nat) (b : vec Type (S n) -> Type) : ctx -> Type :=
-    | nnil : ngenv b nil
+  (* env of terms of kind-indexed types
+     Needed for constructing specialized terms. *)
+  Inductive stenv (n : nat) (b : vec Type (S n) -> Type) : ctx -> Type :=
+    | nnil : stenv b nil
     | ncons : forall {k} {G} (a : vec (decodeKind k) (S n)),
-        kit k b a -> ngenv b G -> ngenv b (cons k G).
+        kit k b a -> stenv b G -> stenv b (cons k G).
 
   (* interpret a generic type + vector of envs to a vec of types *)
-  Definition interp' (G : ctx) (k : kind) (n : nat)
+  Definition interpToVec (G : ctx) (k : kind) (n : nat)
     : typ G k -> vec (env G) n -> vec (decodeKind k) n :=
     fun t vs =>
       zap (repeat _ (decodeType t)) vs.
 
-  (* kit equality *)
+  (* if two types are equal then kit t1 implies kit t2 *)
   Definition eqkit : forall (n : nat) (k : kind) (b : vec Type (S n) -> Type)
     (t1 t2 : vec (decodeKind k) (S n)),
     t1 = t2 -> kit k b t1 -> kit k b t2.
@@ -49,17 +63,18 @@ Section terms.
     intros. induction H; assumption.
   Defined.
 
-  (* turn an ngenv to a vector of envs *)
+  (* turn an stenv to a vector of envs *)
   (* use '@' to provide implicits explicitly *)
   Fixpoint transpose {n : nat} {b : vec Type (S n) -> Type}
-    {G : ctx} (nge : ngenv b G)
+    {G : ctx} (ste : stenv b G)
     : vec (env G) (S n) :=
-      match nge with
+      match ste with
       | nnil _ => repeat _ enil
-      | ncons a _ nge => zap (zap (repeat _ (@econs _ _)) a) (transpose nge)
+      | ncons a _ ste => zap (zap (repeat _ (@econs _ _)) a) (transpose ste)
       end.
 
-  (* PROOFS to help with term specialization, definitions from W + C *)
+  (* PROOFS to help with term specialization,
+     type signatures from definitions by Weirich + Casinghino. *)
 
   (* helper *)
   Lemma eqtail : forall {A} (n : nat) (t1 t2 : vec A n) (x : A),
@@ -67,6 +82,8 @@ Section terms.
   Proof.
     intros A n t1 t2 x eq. rewrite eq. reflexivity.
   Defined.
+
+  (* six lemmas for typechecking different cases of generic types in specTerm  *)
 
   Lemma c6 : forall (n : nat) (A B : Type) (f : A -> B) (x : A),
     zap (repeat n f) (repeat n x) = repeat n (f x).
@@ -78,7 +95,7 @@ Section terms.
 
   Lemma c5 : forall (n : nat) (k : kind) (G : ctx) (c : const k)
     (envs : vec (env G) n),
-      repeat n (decodeClosed (Con _ c)) = interp' (Con _ c) envs.
+      repeat n (decodeClosed (Con _ c)) = interpToVec (Con _ c) envs.
   Proof.
     intros n k G c envs. induction envs.
     - simpl. destruct G.
@@ -93,7 +110,7 @@ Section terms.
     (t1 : typ G (F k1 k2))
     (t2 : typ G k1)
     (envs : vec (env G) n),
-    zap (interp' t1 envs) (interp' t2 envs) = interp' (App t1 t2) envs.
+    zap (interpToVec t1 envs) (interpToVec t2 envs) = interpToVec (App t1 t2) envs.
   Proof.
     intros n k1 k2 G t1 t2 envs. generalize dependent G.
     induction envs.
@@ -101,14 +118,14 @@ Section terms.
       + simpl. reflexivity.
       + simpl. reflexivity.
     -  destruct a.
-      + simpl. apply eqtail. unfold interp' in IHenvs. apply IHenvs.
-      + simpl. apply eqtail. unfold interp' in IHenvs. apply IHenvs.
+      + simpl. apply eqtail. unfold interpToVec in IHenvs. apply IHenvs.
+      + simpl. apply eqtail. unfold interpToVec in IHenvs. apply IHenvs.
   Defined.
 
   Lemma c3 : forall (n : nat) (k k' : kind) (G : ctx)
     (t : typ (cons k' G) k) (envs : vec (env G) n) (As : vec (decodeKind k') n),
-    interp' t (zap (zap (repeat n (@econs k' G)) As) envs)
-    = zap (interp' (Lam t) envs) As.
+    interpToVec t (zap (zap (repeat n (@econs k' G)) As) envs)
+    = zap (interpToVec (Lam t) envs) As.
   Proof.
     intros. destruct n.
     - induction envs eqn:An.
@@ -130,8 +147,8 @@ Section terms.
 
   Lemma c2 : forall (n : nat) (k k' : kind) (G : ctx)
     (x : tyvar G k') (t1 : vec (decodeKind k) n) (envs : vec (env G) n),
-    interp' (Var x) envs
-    = interp' (Var (Vs _ x)) (zap (zap (repeat n (@econs _ _)) t1) envs).
+    interpToVec (Var x) envs
+    = interpToVec (Var (Vs _ x)) (zap (zap (repeat n (@econs _ _)) t1) envs).
   Proof.
     intros. induction envs.
     - simpl. destruct G.
@@ -144,60 +161,60 @@ Section terms.
 
   Lemma c1 : forall (n : nat) (k : kind) (G : ctx)
     (a : vec (decodeKind k) n) (envs : vec (env G) n),
-    a = interp' (Var (Vz _ _)) (zap (zap (repeat n (@econs _ _)) a) envs).
+    a = interpToVec (Var (Vz _ _)) (zap (zap (repeat n (@econs _ _)) a) envs).
   Proof.
     intros. induction a.
     - simpl. reflexivity.
     - apply eqtail. apply IHa.
   Defined.
 
-  (** Lookup a type for var from nge.
+  (** Lookup a type for var from stenv.
       Requires a self defined lemma 'tvcase' for destructing v.
       Done following the idea presented by James Wilcox in:
       - https://jamesrwilcox.com/dep-destruct.html              **)
   Fixpoint nlookup (n : nat) (k : kind) (b : vec Type (S n) -> Type) (G : ctx)
-    (v : tyvar G k) (nge : ngenv b G) :
-    kit k b (interp' (Var v) (transpose nge)).
+    (v : tyvar G k) (ste : stenv b G) :
+    kit k b (interpToVec (Var v) (transpose ste)).
   Proof.
-    destruct nge.
+    destruct ste.
     - inversion v.
     - pattern v; apply tvcase; clear v; intros.
       + subst. apply eqkit with (t1:=a).
-        * pose proof (c1 _ a (transpose nge)) as ch. simpl in ch; simpl.
+        * pose proof (c1 _ a (transpose ste)) as ch. simpl in ch; simpl.
           rewrite <- ch; reflexivity.
         * assumption.
-      + pose proof (c2 _ x a (transpose nge)) as ch.
+      + pose proof (c2 _ x a (transpose ste)) as ch.
         apply eqkit with (b:=b) in ch.
         * apply ch.
-       * exact (nlookup _ _ _ _ x nge). Defined.
+       * exact (nlookup _ _ _ _ x ste). Defined.
 
   (* term specialization with non-empty context *)
-  Fixpoint ngen' (n : nat) (b : vec Type (S n) -> Type)
+  Fixpoint specTerm' (n : nat) (b : vec Type (S n) -> Type)
     (G : ctx) (k : kind) (t : typ G k)
-    : forall (ve : ngenv b G) (ce : tyConstEnv b),
-    kit k b (interp' t (transpose ve)) :=
+    : forall (ve : stenv b G) (ce : tyConstEnv b),
+    kit k b (interpToVec t (transpose ve)) :=
     match t in typ G k
-    return forall (ve : ngenv b G) (ce : tyConstEnv b),
-    kit k b (interp' t (transpose ve)) with
+    return forall (ve : stenv b G) (ce : tyConstEnv b),
+    kit k b (interpToVec t (transpose ve)) with
     | Var x => fun ve ce => nlookup x ve
     | @Lam _ k1 k2 t1 => fun ve ce =>
         curry _ (fun (a : vec (decodeKind k1) (S n)) (nwt : kit k1 b a) =>
                   eqkit _ _ (c3 t1 (transpose ve) a)
-                  (ngen' t1 (ncons a nwt ve) ce))
+                  (specTerm' t1 (ncons a nwt ve) ce))
     | @App _ k1 k2 t1 t2 => fun ve ce =>
         eqkit _ _ (c4 t1 t2 (transpose ve))
         (@uncurry' (S n) (decodeKind k1) (fun a => (forall _: kit k1 b a,
-                       (kit k2 b (zap (interp' t1 (transpose ve)) a))))
-        (@ngen' _ _ _ (F k1 k2) t1 ve ce)
-        (interp' t2 (transpose ve)) (ngen' t2 ve ce)
+                       (kit k2 b (zap (interpToVec t1 (transpose ve)) a))))
+        (@specTerm' _ _ _ (F k1 k2) t1 ve ce)
+        (interpToVec t2 (transpose ve)) (specTerm' t2 ve ce)
         )
     | Con _ c => fun ve ce => eqkit _ _ (c5 c (transpose ve)) (ce _ c)
     end.
 
   (* term specialization in an empty context. *)
-  Definition ngen (n : nat) (b : vec Type (S n) -> Type) (k : kind) (t : ty k)
+  Definition specTerm (n : nat) (b : vec Type (S n) -> Type) (k : kind) (t : ty k)
   (ce : tyConstEnv b) : kit k b (repeat (S n) (decodeClosed t)) :=
-  eqkit k b (c6 _ _ _ ) (ngen' t (nnil _) ce).
+  eqkit k b (c6 _ _ _ ) (specTerm' t (nnil _) ce).
 
 End terms.
 
